WIP: proving produces and drops inv

dataplane/Correctness/General.thy
@@ -75,7 +75,7 @@ lemma inputs_at_target_consumes[simp]:
 definition "ty1_check os bufs = (\<forall> p. (\<forall> x \<in> fst ` set (input os p) \<union> fst ` set (bufs p) \<union> fst ` set (outpu os p). is_en1 os x))"
 definition "ty2_check os bufs = (\<forall> p. (\<forall> x \<in> fst ` set (input os p) \<union> fst ` set (bufs p). is_en1 os x) \<and> (\<forall> x \<in> fst ` set (outpu os p). is_en2 os x))"
 
-definition "produ_consu_supported nt os c =
+definition "produ_consu_inter_supported nt os c =
     ((\<forall> nid p t m. (p, t, m) \<in> set (produ (os nid)) \<longrightarrow> (zcount (c_pts c (Loc nid (Src p))) t > 0 \<or> (\<exists>m'>0. (p, t, m') \<in> set (inter (os nid))))) \<and>
      (\<forall> nid p t m. (p, t, m) \<in> set (consu (os nid)) \<longrightarrow>
                    (zcount (c_pts c (Loc nid (Trg p)) + zmset (concat (map (\<lambda> (nid', p'). (map snd (filter (\<lambda> (p'', _, _). nt (nid', p'') = Some (nid, p) \<and> p' = p'') (produ (os nid'))))) Enum.enum))) t > 0)) \<and>
@@ -101,7 +101,7 @@ definition "dataplane_tracker_inv os cbufs sg =
      change_deltas_inv os \<and>
      propagation_inv (summ sg) c \<and>
      extract_prog_changes_above_impl_inv (summ sg) (nxt sg) c os  \<and>
-     (produ_consu_supported (nxt sg) os c))"
+     (produ_consu_inter_supported (nxt sg) os c))"
 
 
 definition "graph_summar_nt su nt os = (
